src/3d/Batch.fsti
@@ -2,6 +2,8 @@ module Batch
 open FStar.All
 
 val postprocess
+  (clang_format: bool)
+  (clang_format_executable: string)
   (out_dir: string)
   (files_and_modules: list (string & string))
 : ML unit
